A12Kernel/Proofs.lean
@@ -164,6 +164,7 @@ import A12Kernel.Proofs.BooleanFirstFilledComputation
 import A12Kernel.Proofs.CustomFirstFilledComputation
 import A12Kernel.Proofs.DateFragmentFirstFilledComputation
 import A12Kernel.Proofs.FullDateFirstFilledComputation
+import A12Kernel.Proofs.TimeFirstFilledComputation
 import A12Kernel.Proofs.TokenFirstFilledValue
 import A12Kernel.Proofs.StarCompleteness
 import A12Kernel.Proofs.StarAddressing
